secure_api/box/functor_box/Box.PKAE.fst
@@ -44,6 +44,9 @@ let length = AE.length
 let pkey = ODH.pkey
 let skey = ODH.skey
 
+let pkey_from_skey sk = ODH.get_pkey sk
+let compatible_keys sk pk = ODH.compatible_keys sk pk
+
 #set-options "--z3rlimit 900 --max_ifuel 2 --max_fuel 1"
 private noeq type aux_t' (im:index_module{ID.get_subId im == subId_t}) (pm:plain_module) (rgn:log_region im) =
   | AUX:
@@ -85,15 +88,24 @@ let get_message_logGT pkm =
   let log:message_log pkm.im ae_rgn = coerce (AE.message_log pkm.im ae_rgn) (message_log pkm.im ae_rgn) ae_log in
   log
 
-val create_aux: (im:index_module{ID.get_subId im == subId_t}) -> (pm:plain_module{Plain.get_plain pm == plain_t}) -> rgn:log_region im -> St (aux_t im pm rgn)
+val create_aux: (im:index_module{ID.get_subId im == subId_t}) -> (pm:plain_module{Plain.get_plain pm == plain_t /\ Plain.plain_max_length #pm == plain_max_length}) -> rgn:log_region im -> St (aux_t im pm rgn)
 let create_aux im pm rgn =
   let am = AE.create im pm rgn in
   let km = AE.instantiate_km am in
   let om = ODH.create im km rgn in
   AUX am km om
 
-assume val enc (pm:plain_module): (Plain.get_plain pm) -> n:nonce -> pk:pkey -> sk:skey -> Tot cipher
-assume val dec (pm:plain_module): c:cipher -> n:nonce -> pk:pkey -> sk:skey -> Tot (option (Plain.get_plain pm)) 
+  
+assume val lemma_compatible_length: n:nat -> Lemma
+  (requires n < plain_max_length)
+  (ensures n / Spec.Salsa20.blocklen < pow2 32)
+
+val enc (im:ODH.index_module): plain_t -> n:nonce -> pk:pkey -> sk:skey{ODH.compatible_keys sk pk} -> GTot cipher
+let enc im p n pk sk = 
+  lemma_compatible_length (length p);
+  SPEC.secretbox_easy p (ODH.prf_odhGT im sk pk) n
+
+assume val dec: c:cipher -> n:nonce -> pk:pkey -> sk:skey -> Tot (option plain_t) 
 
 let create rgn =
   let id_log_rgn : ID.id_log_region = new_region rgn in
@@ -101,7 +113,7 @@ let create rgn =
   let pm = Plain.create plain_t AE.plain_max_length AE.length in
   let log_rgn : log_region im = new_region rgn in
   let aux = create_aux im pm log_rgn in
-  PKAE im pm log_rgn (enc pm) (dec pm) aux
+  PKAE im pm log_rgn (enc im) (dec) aux
 
 
 type key (pkm:pkae_module) = AE.key pkm.im
@@ -114,20 +126,15 @@ let pkey_to_subId_inj #pkm pk = ODH.lemma_pk_get_share_inj pk
 let nonce_is_fresh (pkm:pkae_module) (i:id pkm.im) (n:nonce) (h:mem) =
   AE.nonce_is_fresh pkm.aux.am i n h
 
-let pkey_from_skey sk = ODH.get_pkey sk
 
 let gen pkm =
   ODH.keygen()
-
-let compatible_keys sk pk = ODH.compatible_keys sk pk
-
-
 
 #set-options "--z3rlimit 500 --max_ifuel 0 --max_fuel 0"
 let encrypt pkm #i n sk pk m =
   let k = ODH.prf_odh pkm.im pkm.aux.km pkm.aux.om sk pk in
   let c = AE.encrypt pkm.aux.am #i n k m in
-  let h = get() in
+    let h = get() in
   assert(FStar.FunctionalExtensionality.feq (message_log_range pkm.im) (AE.message_log_range pkm.im));
   MM.contains_eq_compat (get_message_logGT pkm) (AE.get_message_logGT pkm.aux.am) (n,i) (c,m) h;
   MM.contains_stable (get_message_logGT pkm) (n,i) (c,m);
@@ -135,6 +142,6 @@ let encrypt pkm #i n sk pk m =
   c
 
 let decrypt pkm #i n sk pk c =
-  let k = ODH.prf_odh pkm.im pkm.km pkm.om sk pk in
-  let m = AE.decrypt pkm.am #i n k c in
+  let k = ODH.prf_odh pkm.im pkm.aux.km pkm.aux.om sk pk in
+  let m = AE.decrypt pkm.aux.am #i n k c in
   m
